theories/program_logic/ectx_lifting.v
@@ -12,61 +12,93 @@ Implicit Types v : val.
 Implicit Types e : expr.
 Hint Resolve head_prim_reducible head_reducible_prim_step.
 
-Lemma wp_ectx_bind {E Φ} K e :
-  WP e @ E {{ v, WP fill K (of_val v) @ E {{ Φ }} }} ⊢ WP fill K e @ E {{ Φ }}.
+Definition head_progressive (e : expr) (σ : state) :=
+  is_Some(to_val e) ∨ ∃ K e', e = fill K e' ∧ head_reducible e' σ.
+
+Lemma progressive_head_progressive e σ :
+  progressive e σ → head_progressive e σ.
+Proof.
+  case=>[?|Hred]; first by left.
+  right. move: Hred=> [] e' [] σ' [] efs [] K e1' e2' EQ EQ' Hstep. subst.
+  exists K, e1'. split; first done. by exists e2', σ', efs.
+Qed.
+Hint Resolve progressive_head_progressive.
+
+Lemma wp_ectx_bind {p E e} K Φ :
+  WP e @ p; E {{ v, WP fill K (of_val v) @ p; E {{ Φ }} }} ⊢ WP fill K e @ p; E {{ Φ }}.
 Proof. apply: weakestpre.wp_bind. Qed.
 
-Lemma wp_ectx_bind_inv {E Φ} K e :
-  WP fill K e @ E {{ Φ }} ⊢ WP e @ E {{ v, WP fill K (of_val v) @ E {{ Φ }} }}.
+Lemma wp_ectx_bind_inv {p E Φ} K e :
+  WP fill K e @ p; E {{ Φ }} ⊢ WP e @ p; E {{ v, WP fill K (of_val v) @ p; E {{ Φ }} }}.
 Proof. apply: weakestpre.wp_bind_inv. Qed.
 
-Lemma wp_lift_head_step {E Φ} e1 :
+Lemma wp_lift_head_step {p E Φ} e1 :
   to_val e1 = None →
   (∀ σ1, state_interp σ1 ={E,∅}=∗
     ⌜head_reducible e1 σ1⌝ ∗
     ▷ ∀ e2 σ2 efs, ⌜head_step e1 σ1 e2 σ2 efs⌝ ={∅,E}=∗
-      state_interp σ2 ∗ WP e2 @ E {{ Φ }} ∗ [∗ list] ef ∈ efs, WP ef {{ _, True }})
-  ⊢ WP e1 @ E {{ Φ }}.
+      state_interp σ2 ∗ WP e2 @ p; E {{ Φ }} ∗ [∗ list] ef ∈ efs, WP ef @ p; ⊤ {{ _, True }})
+  ⊢ WP e1 @ p; E {{ Φ }}.
 Proof.
-  iIntros (?) "H". iApply (wp_lift_step E)=>//. iIntros (σ1) "Hσ".
+  iIntros (?) "H". iApply wp_lift_step=>//. iIntros (σ1) "Hσ".
   iMod ("H" $! σ1 with "Hσ") as "[% H]"; iModIntro.
   iSplit; first by eauto. iNext. iIntros (e2 σ2 efs) "%".
   iApply "H". by eauto.
 Qed.
 
-Lemma wp_lift_pure_head_step {E E' Φ} e1 :
+Lemma wp_lift_head_stuck E Φ e :
+  to_val e = None →
+  (∀ σ, state_interp σ ={E,∅}=∗ ⌜¬ head_progressive e σ⌝)
+  ⊢ WP e @ E ?{{ Φ }}.
+Proof.
+  iIntros (?) "H". iApply wp_lift_stuck; first done.
+  iIntros (σ) "Hσ". iMod ("H" $! _ with "Hσ") as "%". iModIntro. by auto.
+Qed.
+
+Lemma wp_lift_pure_head_step {p E E' Φ} e1 :
   (∀ σ1, head_reducible e1 σ1) →
   (∀ σ1 e2 σ2 efs, head_step e1 σ1 e2 σ2 efs → σ1 = σ2) →
   (|={E,E'}▷=> ∀ e2 efs σ, ⌜head_step e1 σ e2 σ efs⌝ →
-    WP e2 @ E {{ Φ }} ∗ [∗ list] ef ∈ efs, WP ef {{ _, True }})
-  ⊢ WP e1 @ E {{ Φ }}.
+    WP e2 @ p; E {{ Φ }} ∗ [∗ list] ef ∈ efs, WP ef @ p; ⊤ {{ _, True }})
+  ⊢ WP e1 @ p; E {{ Φ }}.
 Proof using Hinh.
   iIntros (??) "H". iApply wp_lift_pure_step; eauto.
   iApply (step_fupd_wand with "H"); iIntros "H".
   iIntros (????). iApply "H"; eauto.
 Qed.
 
-Lemma wp_lift_atomic_head_step {E Φ} e1 :
+Lemma wp_lift_pure_head_stuck `{Inhabited state} E Φ e :
+  to_val e = None →
+  (∀ K e1 σ1 e2 σ2 efs, e = fill K e1 → ¬ head_step e1 σ1 e2 σ2 efs) →
+  WP e @ E ?{{ Φ }}%I.
+Proof.
+  iIntros (Hnv Hnstep). iApply wp_lift_head_stuck; first done.
+  iIntros (σ) "_". iMod (fupd_intro_mask' E ∅) as "_"; first set_solver.
+  iModIntro. iPureIntro. case; first by rewrite Hnv; case.
+  move=>[] K [] e1 [] Hfill [] e2 [] σ2 [] efs /= Hstep. exact: Hnstep.
+Qed.
+
+Lemma wp_lift_atomic_head_step {p E Φ} e1 :
   to_val e1 = None →
   (∀ σ1, state_interp σ1 ={E}=∗
     ⌜head_reducible e1 σ1⌝ ∗
     ▷ ∀ e2 σ2 efs, ⌜head_step e1 σ1 e2 σ2 efs⌝ ={E}=∗
       state_interp σ2 ∗
-      default False (to_val e2) Φ ∗ [∗ list] ef ∈ efs, WP ef {{ _, True }})
-  ⊢ WP e1 @ E {{ Φ }}.
+      default False (to_val e2) Φ ∗ [∗ list] ef ∈ efs, WP ef @ p; ⊤ {{ _, True }})
+  ⊢ WP e1 @ p; E {{ Φ }}.
 Proof.
   iIntros (?) "H". iApply wp_lift_atomic_step; eauto.
   iIntros (σ1) "Hσ1". iMod ("H" $! σ1 with "Hσ1") as "[% H]"; iModIntro.
   iSplit; first by eauto. iNext. iIntros (e2 σ2 efs) "%". iApply "H"; auto.
 Qed.
 
-Lemma wp_lift_atomic_head_step_no_fork {E Φ} e1 :
+Lemma wp_lift_atomic_head_step_no_fork {p E Φ} e1 :
   to_val e1 = None →
   (∀ σ1, state_interp σ1 ={E}=∗
     ⌜head_reducible e1 σ1⌝ ∗
     ▷ ∀ e2 σ2 efs, ⌜head_step e1 σ1 e2 σ2 efs⌝ ={E}=∗
       ⌜efs = []⌝ ∗ state_interp σ2 ∗ default False (to_val e2) Φ)
-  ⊢ WP e1 @ E {{ Φ }}.
+  ⊢ WP e1 @ p; E {{ Φ }}.
 Proof.
   iIntros (?) "H". iApply wp_lift_atomic_head_step; eauto.
   iIntros (σ1) "Hσ1". iMod ("H" $! σ1 with "Hσ1") as "[$ H]"; iModIntro.
@@ -74,32 +106,32 @@ Proof.
   iMod ("H" $! v2 σ2 efs with "[# //]") as "(% & $ & $)"; subst; auto.
 Qed.
 
-Lemma wp_lift_pure_det_head_step {E E' Φ} e1 e2 efs :
+Lemma wp_lift_pure_det_head_step {p E E' Φ} e1 e2 efs :
   (∀ σ1, head_reducible e1 σ1) →
   (∀ σ1 e2' σ2 efs',
     head_step e1 σ1 e2' σ2 efs' → σ1 = σ2 ∧ e2 = e2' ∧ efs = efs') →
-  (|={E,E'}▷=> WP e2 @ E {{ Φ }} ∗ [∗ list] ef ∈ efs, WP ef {{ _, True }})
-  ⊢ WP e1 @ E {{ Φ }}.
+  (|={E,E'}▷=> WP e2 @ p; E {{ Φ }} ∗ [∗ list] ef ∈ efs, WP ef @ p; ⊤ {{ _, True }})
+  ⊢ WP e1 @ p; E {{ Φ }}.
 Proof using Hinh. eauto using wp_lift_pure_det_step. Qed.
 
-Lemma wp_lift_pure_det_head_step_no_fork {E E' Φ} e1 e2 :
+Lemma wp_lift_pure_det_head_step_no_fork {p E E' Φ} e1 e2 :
   to_val e1 = None →
   (∀ σ1, head_reducible e1 σ1) →
   (∀ σ1 e2' σ2 efs',
     head_step e1 σ1 e2' σ2 efs' → σ1 = σ2 ∧ e2 = e2' ∧ [] = efs') →
-  (|={E,E'}▷=> WP e2 @ E {{ Φ }}) ⊢ WP e1 @ E {{ Φ }}.
+  (|={E,E'}▷=> WP e2 @ p; E {{ Φ }}) ⊢ WP e1 @ p; E {{ Φ }}.
 Proof using Hinh.
   intros. rewrite -(wp_lift_pure_det_step e1 e2 []) /= ?right_id; eauto.
 Qed.
 
-Lemma wp_lift_pure_det_head_step_no_fork' {E Φ} e1 e2 :
+Lemma wp_lift_pure_det_head_step_no_fork' {p E Φ} e1 e2 :
   to_val e1 = None →
   (∀ σ1, head_reducible e1 σ1) →
   (∀ σ1 e2' σ2 efs',
     head_step e1 σ1 e2' σ2 efs' → σ1 = σ2 ∧ e2 = e2' ∧ [] = efs') →
-  ▷ WP e2 @ E {{ Φ }} ⊢ WP e1 @ E {{ Φ }}.
+  ▷ WP e2 @ p; E {{ Φ }} ⊢ WP e1 @ p; E {{ Φ }}.
 Proof using Hinh.
-  intros. rewrite -[(WP e1 @ _ {{ _ }})%I]wp_lift_pure_det_head_step_no_fork //.
+  intros. rewrite -[(WP e1 @ _; _ {{ _ }})%I]wp_lift_pure_det_head_step_no_fork //.
   rewrite -step_fupd_intro //.
 Qed.
 End wp.
