theories/program_logic/hoare.v
@@ -3,24 +3,42 @@ From iris.base_logic.lib Require Export viewshifts.
 From iris.proofmode Require Import tactics.
 Set Default Proof Using "Type".
 
-Definition ht `{irisG Λ Σ} (E : coPset) (P : iProp Σ)
+Definition ht `{irisG Λ Σ} (p : bool) (E : coPset) (P : iProp Σ)
     (e : expr Λ) (Φ : val Λ → iProp Σ) : iProp Σ :=
-  (□ (P -∗ WP e @ E {{ Φ }}))%I.
-Instance: Params (@ht) 4.
+  (□ (P -∗ WP e @ p; E {{ Φ }}))%I.
+Instance: Params (@ht) 5.
 
-Notation "{{ P } } e @ E {{ Φ } }" := (ht E P%I e%E Φ%I)
+Notation "{{ P } } e @ p ; E {{ Φ } }" := (ht p E P%I e%E Φ%I)
+  (at level 20, P, e, Φ at level 200,
+   format "{{  P  } }  e  @  p ;  E  {{  Φ  } }") : C_scope.
+Notation "{{ P } } e @ E {{ Φ } }" := (ht true E P%I e%E Φ%I)
   (at level 20, P, e, Φ at level 200,
    format "{{  P  } }  e  @  E  {{  Φ  } }") : C_scope.
-Notation "{{ P } } e {{ Φ } }" := (ht ⊤ P%I e%E Φ%I)
+Notation "{{ P } } e @ E ? {{ Φ } }" := (ht false E P%I e%E Φ%I)
+  (at level 20, P, e, Φ at level 200,
+   format "{{  P  } }  e  @  E  ? {{  Φ  } }") : C_scope.
+Notation "{{ P } } e {{ Φ } }" := (ht true ⊤ P%I e%E Φ%I)
   (at level 20, P, e, Φ at level 200,
    format "{{  P  } }  e  {{  Φ  } }") : C_scope.
+Notation "{{ P } } e ? {{ Φ } }" := (ht false ⊤ P%I e%E Φ%I)
+  (at level 20, P, e, Φ at level 200,
+   format "{{  P  } }  e  ? {{  Φ  } }") : C_scope.
 
-Notation "{{ P } } e @ E {{ v , Q } }" := (ht E P%I e%E (λ v, Q)%I)
+Notation "{{ P } } e @ p ; E {{ v , Q } }" := (ht p E P%I e%E (λ v, Q)%I)
+  (at level 20, P, e, Q at level 200,
+   format "{{  P  } }  e  @  p ;  E  {{  v ,  Q  } }") : C_scope.
+Notation "{{ P } } e @ E {{ v , Q } }" := (ht true E P%I e%E (λ v, Q)%I)
   (at level 20, P, e, Q at level 200,
    format "{{  P  } }  e  @  E  {{  v ,  Q  } }") : C_scope.
-Notation "{{ P } } e {{ v , Q } }" := (ht ⊤ P%I e%E (λ v, Q)%I)
+Notation "{{ P } } e @ E ? {{ v , Q } }" := (ht false E P%I e%E (λ v, Q)%I)
+  (at level 20, P, e, Q at level 200,
+   format "{{  P  } }  e  @  E  ? {{  v ,  Q  } }") : C_scope.
+Notation "{{ P } } e {{ v , Q } }" := (ht true ⊤ P%I e%E (λ v, Q)%I)
   (at level 20, P, e, Q at level 200,
    format "{{  P  } }  e  {{  v ,  Q  } }") : C_scope.
+Notation "{{ P } } e ? {{ v , Q } }" := (ht false ⊤ P%I e%E (λ v, Q)%I)
+  (at level 20, P, e, Q at level 200,
+   format "{{  P  } }  e  ? {{  v ,  Q  } }") : C_scope.
 
 Section hoare.
 Context `{irisG Λ Σ}.
@@ -29,100 +47,106 @@ Implicit Types Φ Ψ : val Λ → iProp Σ.
 Implicit Types v : val Λ.
 Import uPred.
 
-Global Instance ht_ne E n :
-  Proper (dist n ==> eq ==> pointwise_relation _ (dist n) ==> dist n) (ht E).
+Global Instance ht_ne p E n :
+  Proper (dist n ==> eq ==> pointwise_relation _ (dist n) ==> dist n) (ht p E).
 Proof. solve_proper. Qed.
-Global Instance ht_proper E :
-  Proper ((≡) ==> eq ==> pointwise_relation _ (≡) ==> (≡)) (ht E).
+Global Instance ht_proper p E :
+  Proper ((≡) ==> eq ==> pointwise_relation _ (≡) ==> (≡)) (ht p E).
 Proof. solve_proper. Qed.
-Lemma ht_mono E P P' Φ Φ' e :
-  (P ⊢ P') → (∀ v, Φ' v ⊢ Φ v) → {{ P' }} e @ E {{ Φ' }} ⊢ {{ P }} e @ E {{ Φ }}.
+Lemma ht_mono p E P P' Φ Φ' e :
+  (P ⊢ P') → (∀ v, Φ' v ⊢ Φ v) → {{ P' }} e @ p; E {{ Φ' }} ⊢ {{ P }} e @ p; E {{ Φ }}.
 Proof. by intros; apply persistently_mono, wand_mono, wp_mono. Qed.
-Global Instance ht_mono' E :
-  Proper (flip (⊢) ==> eq ==> pointwise_relation _ (⊢) ==> (⊢)) (ht E).
+Global Instance ht_mono' p E :
+  Proper (flip (⊢) ==> eq ==> pointwise_relation _ (⊢) ==> (⊢)) (ht p E).
 Proof. solve_proper. Qed.
 
-Lemma ht_alt E P Φ e : (P ⊢ WP e @ E {{ Φ }}) → {{ P }} e @ E {{ Φ }}.
+Lemma ht_alt p E P Φ e : (P ⊢ WP e @ p; E {{ Φ }}) → {{ P }} e @ p; E {{ Φ }}.
 Proof. iIntros (Hwp) "!# HP". by iApply Hwp. Qed.
 
-Lemma ht_val E v : {{ True }} of_val v @ E {{ v', ⌜v = v'⌝ }}.
+Lemma ht_val p E v : {{ True }} of_val v @ p; E {{ v', ⌜v = v'⌝ }}.
 Proof. iIntros "!# _". by iApply wp_value'. Qed.
 
-Lemma ht_vs E P P' Φ Φ' e :
-  (P ={E}=> P') ∧ {{ P' }} e @ E {{ Φ' }} ∧ (∀ v, Φ' v ={E}=> Φ v)
-  ⊢ {{ P }} e @ E {{ Φ }}.
+Lemma ht_vs p E P P' Φ Φ' e :
+  (P ={E}=> P') ∧ {{ P' }} e @ p; E {{ Φ' }} ∧ (∀ v, Φ' v ={E}=> Φ v)
+  ⊢ {{ P }} e @ p; E {{ Φ }}.
 Proof.
   iIntros "(#Hvs & #Hwp & #HΦ) !# HP". iMod ("Hvs" with "HP") as "HP".
   iApply wp_fupd. iApply (wp_wand with "[HP]"); [by iApply "Hwp"|].
   iIntros (v) "Hv". by iApply "HΦ".
 Qed.
 
-Lemma ht_atomic E1 E2 P P' Φ Φ' e :
-  Atomic e →
-  (P ={E1,E2}=> P') ∧ {{ P' }} e @ E2 {{ Φ' }} ∧ (∀ v, Φ' v ={E2,E1}=> Φ v)
-  ⊢ {{ P }} e @ E1 {{ Φ }}.
+Lemma ht_atomic p E1 E2 P P' Φ Φ' e :
+  StronglyAtomic e →
+  (P ={E1,E2}=> P') ∧ {{ P' }} e @ p; E2 {{ Φ' }} ∧ (∀ v, Φ' v ={E2,E1}=> Φ v)
+  ⊢ {{ P }} e @ p; E1 {{ Φ }}.
 Proof.
-  iIntros (?) "(#Hvs & #Hwp & #HΦ) !# HP". iApply (wp_atomic _ E2); auto.
+  iIntros (?) "(#Hvs & #Hwp & #HΦ) !# HP". iApply (wp_atomic _ _ E2); auto.
   iMod ("Hvs" with "HP") as "HP". iModIntro.
   iApply (wp_wand with "[HP]"); [by iApply "Hwp"|].
   iIntros (v) "Hv". by iApply "HΦ".
 Qed.
 
-Lemma ht_bind `{LanguageCtx Λ K} E P Φ Φ' e :
-  {{ P }} e @ E {{ Φ }} ∧ (∀ v, {{ Φ v }} K (of_val v) @ E {{ Φ' }})
-  ⊢ {{ P }} K e @ E {{ Φ' }}.
+Lemma ht_bind `{LanguageCtx Λ K} p E P Φ Φ' e :
+  {{ P }} e @ p; E {{ Φ }} ∧ (∀ v, {{ Φ v }} K (of_val v) @ p; E {{ Φ' }})
+  ⊢ {{ P }} K e @ p; E {{ Φ' }}.
 Proof.
   iIntros "[#Hwpe #HwpK] !# HP". iApply wp_bind.
   iApply (wp_wand with "[HP]"); [by iApply "Hwpe"|].
   iIntros (v) "Hv". by iApply "HwpK".
 Qed.
 
-Lemma ht_mask_weaken E1 E2 P Φ e :
-  E1 ⊆ E2 → {{ P }} e @ E1 {{ Φ }} ⊢ {{ P }} e @ E2 {{ Φ }}.
+Lemma ht_forget_progress E P Φ e :
+  {{ P }} e @ E {{ Φ }} ⊢ {{ P }} e @ E ?{{ Φ }}.
 Proof.
-  iIntros (?) "#Hwp !# HP". iApply (wp_mask_mono E1 E2); try done.
+  by iIntros "#Hwp !# ?"; iApply wp_forget_progress; iApply "Hwp".
+Qed.
+
+Lemma ht_mask_weaken p E1 E2 P Φ e :
+  E1 ⊆ E2 → {{ P }} e @ p; E1 {{ Φ }} ⊢ {{ P }} e @ p; E2 {{ Φ }}.
+Proof.
+  iIntros (?) "#Hwp !# HP". iApply (wp_mask_mono _ E1 E2); try done.
   by iApply "Hwp".
 Qed.
 
-Lemma ht_frame_l E P Φ R e :
-  {{ P }} e @ E {{ Φ }} ⊢ {{ R ∗ P }} e @ E {{ v, R ∗ Φ v }}.
+Lemma ht_frame_l p E P Φ R e :
+  {{ P }} e @ p; E {{ Φ }} ⊢ {{ R ∗ P }} e @ p; E {{ v, R ∗ Φ v }}.
 Proof. iIntros "#Hwp !# [$ HP]". by iApply "Hwp". Qed.
 
-Lemma ht_frame_r E P Φ R e :
-  {{ P }} e @ E {{ Φ }} ⊢ {{ P ∗ R }} e @ E {{ v, Φ v ∗ R }}.
+Lemma ht_frame_r p E P Φ R e :
+  {{ P }} e @ p; E {{ Φ }} ⊢ {{ P ∗ R }} e @ p; E {{ v, Φ v ∗ R }}.
 Proof. iIntros "#Hwp !# [HP $]". by iApply "Hwp". Qed.
 
-Lemma ht_frame_step_l E1 E2 P R1 R2 e Φ :
+Lemma ht_frame_step_l p E1 E2 P R1 R2 e Φ :
   to_val e = None → E2 ⊆ E1 →
-  (R1 ={E1,E2}=> ▷ |={E2,E1}=> R2) ∧ {{ P }} e @ E2 {{ Φ }}
-  ⊢ {{ R1 ∗ P }} e @ E1 {{ λ v, R2 ∗ Φ v }}.
+  (R1 ={E1,E2}=> ▷ |={E2,E1}=> R2) ∧ {{ P }} e @ p; E2 {{ Φ }}
+  ⊢ {{ R1 ∗ P }} e @ p; E1 {{ λ v, R2 ∗ Φ v }}.
 Proof.
   iIntros (??) "[#Hvs #Hwp] !# [HR HP]".
-  iApply (wp_frame_step_l E1 E2); try done.
+  iApply (wp_frame_step_l _ E1 E2); try done.
   iSplitL "HR"; [by iApply "Hvs"|by iApply "Hwp"].
 Qed.
 
-Lemma ht_frame_step_r E1 E2 P R1 R2 e Φ :
+Lemma ht_frame_step_r p E1 E2 P R1 R2 e Φ :
   to_val e = None → E2 ⊆ E1 →
-  (R1 ={E1,E2}=> ▷ |={E2,E1}=> R2) ∧ {{ P }} e @ E2 {{ Φ }}
-  ⊢ {{ P ∗ R1 }} e @ E1 {{ λ v, Φ v ∗ R2 }}.
+  (R1 ={E1,E2}=> ▷ |={E2,E1}=> R2) ∧ {{ P }} e @ p; E2 {{ Φ }}
+  ⊢ {{ P ∗ R1 }} e @ p; E1 {{ λ v, Φ v ∗ R2 }}.
 Proof.
   iIntros (??) "[#Hvs #Hwp] !# [HP HR]".
-  iApply (wp_frame_step_r E1 E2); try done.
+  iApply (wp_frame_step_r _ E1 E2); try done.
   iSplitR "HR"; [by iApply "Hwp"|by iApply "Hvs"].
 Qed.
 
-Lemma ht_frame_step_l' E P R e Φ :
+Lemma ht_frame_step_l' p E P R e Φ :
   to_val e = None →
-  {{ P }} e @ E {{ Φ }} ⊢ {{ ▷ R ∗ P }} e @ E {{ v, R ∗ Φ v }}.
+  {{ P }} e @ p; E {{ Φ }} ⊢ {{ ▷ R ∗ P }} e @ p; E {{ v, R ∗ Φ v }}.
 Proof.
   iIntros (?) "#Hwp !# [HR HP]".
   iApply wp_frame_step_l'; try done. iFrame "HR". by iApply "Hwp".
 Qed.
 
-Lemma ht_frame_step_r' E P Φ R e :
+Lemma ht_frame_step_r' p E P Φ R e :
   to_val e = None →
-  {{ P }} e @ E {{ Φ }} ⊢ {{ P ∗ ▷ R }} e @ E {{ v, Φ v ∗ R }}.
+  {{ P }} e @ p; E {{ Φ }} ⊢ {{ P ∗ ▷ R }} e @ p; E {{ v, Φ v ∗ R }}.
 Proof.
   iIntros (?) "#Hwp !# [HP HR]".
   iApply wp_frame_step_r'; try done. iFrame "HR". by iApply "Hwp".
